Examples/OMemSpec.v
@@ -1,0 +1,33 @@
+From LHL.Core Require Import
+  Program
+  Specs.
+
+Variant OMemSig {A} : ESig :=
+| Write (x : A) : OMemSig unit
+| Read : OMemSig A.
+Arguments OMemSig : clear implicits.
+
+Variant OMemState {A} :=
+| OMemInit
+| OMemWriteRan (s : A)
+| OMemCanRead (s : A) (m : bool)
+| OMemUB.
+Arguments OMemState : clear implicits.
+
+Notation OMemIdle s := (OMemCanRead s false).
+Notation OMemReadRan s := (OMemCanRead s true).
+
+Variant OMemStep {A} : OMemState A -> ThreadEvent (OMemSig A) -> OMemState A -> Prop :=
+| OMemCallWrite i s :
+  OMemStep OMemInit (i, CallEv (Write s)) (OMemWriteRan s)
+| OMemRetWrite i s :
+  OMemStep (OMemWriteRan s) (i, RetEv (Write s) tt) (OMemIdle s)
+| OMemCallRead i s :
+  OMemStep (OMemIdle s) (i, CallEv Read) (OMemReadRan s)
+| OMemRetRead i s :
+  OMemStep (OMemReadRan s) (i, RetEv Read s) (OMemIdle s)
+| OMemDoubleRead i s t :
+  s <> OMemInit ->
+  OMemStep s (i, CallEv (Write t)) OMemUB
+| OMemStepUB e :
+  OMemStep OMemUB e OMemUB.
