Examples/WriteSnapshot.v
@@ -1,0 +1,22 @@
+From LHL.Core Require Import
+  Program
+  ProgramRules
+  Specs
+  Logic
+  LogicFacts
+  Tensor
+  Traces
+  Linearizability.
+
+From LHL.Examples Require Import
+  OMemSpec
+  WriteSnapshotSpec.
+
+From LHL.Util Require Import
+  Tactics
+  TransUtil
+  Util.
+
+Definition Underlay := OMemSig nat.
+
+Definition write_snapshot : nat 
