Examples/WriteSnapshotSpec.v
@@ -1,0 +1,33 @@
+From LHL.Core Require Import
+  Program
+  Specs.
+
+From LHL.Examples Require Import
+  OMemSpec.
+
+From LHL.Util Require Import
+  Util.
+
+Variant WSSig {A} : ESig :=
+| WS (n : A) : WSSig (list A).
+Arguments WSSig : clear implicits.
+
+Variant WSState {A} :=
+| WSUB
+| WSDef (* change to set *) (vs : list A) (m : ThreadName -> bool).
+Arguments WSState : clear implicits.
+
+Variant WSStep {A} : WSState A -> ThreadEvent (WSSig A) -> WSState A -> Prop :=
+| WSCall i vs v m m' :
+    m i = false ->
+    m' i = true ->
+    differ_pointwise m m' i ->
+    WSStep (WSDef vs m) (i, CallEv (WS v)) (WSDef (cons v vs) m')
+| WSRet i v vs m :
+    m i = true ->
+    WSStep (WSDef vs m) (i, RetEv (WS v) vs) (WSDef vs m)
+| WSDouble i v vs m :
+    m i = true ->
+    WSStep (WSDef vs m) (i, CallEv (WS v)) WSUB
+| WSStepUB e :
+    WSStep WSUB e WSUB.
